Add half solution to 3.9.

BExp.thy
@@ -106,4 +106,46 @@ lemma "ifval (b2ifexp b) s = bval b s"
 lemma "bval (if2bexp b) s = ifval b s"
   by (induction b, auto)
 
+(* Exercise 3.9 *)
+datatype pbexp =
+  Var vname
+| Neg pbexp
+| And pbexp pbexp
+| Or pbexp pbexp
+
+(* For the purely boolean expressions,
+   variables range over values of type bool. *)
+fun pbval :: "pbexp \<Rightarrow> (vname \<Rightarrow> bool) \<Rightarrow> bool" where
+  "pbval (Var x) s = s x"
+| "pbval (Neg b) s = (\<not> pbval b s)"
+| "pbval (And b1 b2) s = (pbval b1 s \<and> pbval b2 s)"
+| "pbval (Or b1 b2) s = (pbval b1 s \<or> pbval b2 s)"
+
+(* NNF: Negation Normal Form
+   Negation is only applied directly to variables. *)
+fun is_nnf :: "pbexp \<Rightarrow> bool" where
+  "is_nnf (Var _) = True"
+| "is_nnf (Neg (Var _)) = True"
+| "is_nnf (Neg _) = False"
+| "is_nnf (And e1 e2) = (is_nnf e1 \<and> is_nnf e2)"
+| "is_nnf (Or e1 e2) = (is_nnf e1 \<and> is_nnf e2)"
+
+(* Convert pbexp into NNF. *)
+fun nnf :: "pbexp \<Rightarrow> pbexp" where
+  "nnf (Var x) = Var x"
+| "nnf (And e1 e2) = And (nnf e1) (nnf e2)"
+| "nnf (Or e1 e2) = Or (nnf e1) (nnf e2)"
+| "nnf (Neg (Var x)) = Neg (Var x)"
+| "nnf (Neg (Neg b)) = nnf b"
+| "nnf (Neg (And e1 e2)) = Or (nnf (Neg e1)) (nnf (Neg e2))"
+| "nnf (Neg (Or e1 e2)) = And (nnf (Neg e1)) (nnf (Neg e2))"
+
+thm nnf.induct
+
+lemma "is_nnf (nnf b)"
+  by (induction b rule: nnf.induct, auto)
+
+lemma "pbval (nnf b) s = pbval b s"
+  by (induction b rule: nnf.induct, auto)
+
 end
